Foundation/Modal/Hilbert/WeakerThan/K4_KD4.lean
@@ -7,24 +7,25 @@ open Modal.Kripke
 open Formula
 open Formula.Kripke
 
-lemma K4_weakerThan_S4 : (Hilbert.K4 α) ≤ₛ (Hilbert.S4 α) := normal_weakerThan_of_subset $ by intro; aesop;
+lemma K4_weakerThan_KD4 : (Hilbert.K4 α) ≤ₛ (Hilbert.KD4 α) := normal_weakerThan_of_subset $ by intro; aesop;
 
-theorem K4_strictlyWeakerThan_S4 : (Hilbert.K4 ℕ) <ₛ (Hilbert.S4 ℕ) := by
+theorem K4_strictlyWeakerThan_KD4 : (Hilbert.K4 ℕ) <ₛ (Hilbert.KD4 ℕ) := by
   constructor;
-  . exact K4_weakerThan_S4;
+  . exact K4_weakerThan_KD4;
   . apply weakerThan_iff.not.mpr;
     push_neg;
-    use (□(atom 0) ➝ (atom 0));
+    use (□(atom 0) ➝ ◇(atom 0));
     constructor;
     . exact Deduction.maxm! $ by simp;
     . apply K4.Kripke.sound.not_provable_of_countermodel;
-      suffices ∃ F : Frame, Transitive F.Rel ∧ ∃ V : Valuation F, ∃ w : F.World, ¬(Satisfies ⟨F, V⟩ w _) by
+      suffices ∃ F : Frame, Transitive F.Rel ∧ ∃ V : Valuation F, ∃ w : F.World, ¬(Kripke.Satisfies ⟨F, V⟩ w _) by
         simp [ValidOnModel, ValidOnFrame, Satisfies];
         tauto;
-      use ⟨Fin 3, λ _ y => y = 1⟩;
+      let F : Frame := ⟨Fin 1, λ x y => False⟩;
+      use F;
       constructor;
       . simp [Transitive];
-      . use (λ w _ => w = 1), 0;
+      . use (λ w _ => w = 0), 0;
         simp [Semantics.Realize, Satisfies];
 
 end LO.Modal.Hilbert
