Foundation/Modal/Hilbert/WeakerThan/KB5_S5.lean
@@ -1,0 +1,34 @@
+import Foundation.Modal.Kripke.Geach.Systems
+
+namespace LO.Modal.Hilbert
+
+open System
+open Modal.Kripke
+open Formula
+open Formula.Kripke
+
+lemma KB5_weakerThan_S5 : (Hilbert.KB5 ℕ) ≤ₛ (Hilbert.S5 ℕ) := by
+  apply Kripke.weakerThan_of_subset_FrameClass SymmetricEuclideanFrameClass ReflexiveEuclideanFrameClass;
+  rintro F ⟨h_refl, h_eucl⟩;
+  refine ⟨symm_of_refl_eucl h_refl h_eucl, h_eucl⟩;
+
+theorem KB5_strictlyWeakerThan_S5 : (Hilbert.KB5 ℕ) <ₛ (Hilbert.S5 ℕ) := by
+  constructor;
+  . exact KB5_weakerThan_S5;
+  . apply weakerThan_iff.not.mpr;
+    push_neg;
+    use (□(atom 0) ➝ (atom 0));
+    constructor;
+    . exact Deduction.maxm! $ by simp;
+    . apply KB5.Kripke.sound.not_provable_of_countermodel;
+      suffices ∃ F : Frame,  Symmetric F.Rel ∧ Euclidean F.Rel ∧ ∃ V : Valuation F, ∃ w : F.World, ¬(Kripke.Satisfies ⟨F, V⟩ w _) by
+        simp [ValidOnModel, ValidOnFrame, Satisfies];
+        tauto;
+      use ⟨Fin 1, λ x y => False⟩;
+      refine ⟨?_, ?_, ?_⟩;
+      . simp [Symmetric];
+      . simp [Euclidean];
+      . use (λ w _ => False), 0;
+        simp [Satisfies, Semantics.Realize];
+
+end LO.Modal.Hilbert
