Foundation/Modal/Hilbert/WeakerThan/KDB_KTB.lean
@@ -1,0 +1,39 @@
+import Foundation.Modal.Kripke.Geach.Systems
+
+namespace LO.Modal.Hilbert
+
+open System
+open Modal.Kripke
+open Formula
+open Formula.Kripke
+
+lemma KDB_weakerThan_KTB : (Hilbert.KDB ℕ) ≤ₛ (Hilbert.KTB ℕ) := by
+  apply Kripke.weakerThan_of_subset_FrameClass SerialSymmetricFrameClass ReflexiveSymmetricFrameClass;
+  rintro F ⟨F_refl, F_symm⟩;
+  refine ⟨serial_of_refl F_refl, F_symm⟩;
+
+theorem KDB_strictlyWeakerThan_KTB : (Hilbert.KDB ℕ) <ₛ (Hilbert.KTB ℕ) := by
+  constructor;
+  . exact KDB_weakerThan_KTB;
+  . apply weakerThan_iff.not.mpr;
+    push_neg;
+    use (□(atom 0) ➝ (atom 0));
+    constructor;
+    . exact Deduction.maxm! (by simp);
+    . apply KDB.Kripke.sound.not_provable_of_countermodel;
+      suffices ∃ F : Frame, Serial F.Rel ∧ Symmetric F.Rel ∧ ∃ V : Valuation F, ∃ w : F.World, ¬(Satisfies ⟨F, V⟩ w _)  by
+        simp [ValidOnModel, ValidOnFrame, Satisfies];
+        tauto;
+      use ⟨Fin 2, λ x y => x ≠ y⟩;
+      refine ⟨?_, ?_, ?_⟩;
+      . intro x;
+        match x with
+        | 0 => use 1; simp;
+        | 1 => use 0; simp;
+      . unfold Symmetric;
+        tauto;
+      . use (λ x _ => x = 1), 0;
+        simp [Semantics.Realize, Satisfies];
+        omega;
+
+end LO.Modal.Hilbert
